fix hashed_elgamal_generic.ec

examples/hashed_elgamal_generic.ec
@@ -1,12 +1,6 @@
-<<<<<<< HEAD
-require import AllCore FSet List SmtMap CHoareTactic.
+require import AllCore FSet List SmtMap CHoareTactic StdOrder.
 require (*--*) BitWord Distr DInterval.
-(*---*) import StdOrder.RealOrder StdRing.RField StdBigop.Bigint BIA.
-=======
-require import AllCore Int Real FSet StdOrder.
-require (*--*) BitWord Distr DInterval.
-(*---*) import RealOrder RField.
->>>>>>> origin/1.0-preview
+(*---*) import RealOrder RField StdBigop.Bigint BIA.
 require (*--*) DiffieHellman ROM PKE_CPA.
 
 (* The type of plaintexts: bitstrings of length k *)
@@ -86,13 +80,6 @@ module Hashed_ElGamal (H:Hash): Scheme = {
   }
 }.
 
-<<<<<<< HEAD
-clone import ROM.Lazy as ROL with
-  type from  <- group,
-  type to    <- bits,
-  op dsample <- fun (x:group), dbits
-proof * by exact/dbits_ll.
-=======
 clone import ROM as RO with
   type in_t    <- group,
   type out_t   <- bits,
@@ -102,7 +89,6 @@ clone import ROM as RO with
 import Lazy.
 clone import ROM_BadCall as ROC with
   op qH <- qH.
->>>>>>> origin/1.0-preview
 
 clone import FMapCost as FMC with
   type from  <- group.
@@ -114,17 +100,12 @@ module type Adversary (O : POracle) = {
 }.
 
 (* Specializing and merging the hash function *)
-<<<<<<< HEAD
+
 module H = {
   var qs : group list
-  proc init(): unit = { RO.init(); qs <- []; }
-  proc o(x:group): bits = { var y; qs <- x::qs; y <@ RO.o(x); return y; }
-  proc hash = RO.o
-=======
-module H : Hash = {
-  proc init(): unit = { LRO.init(); Log.qs <- fset0; }
-  proc hash(x:group): bits = { var y; y <@ LRO.o(x); return y; }
->>>>>>> origin/1.0-preview
+  proc init(): unit = { LRO.init(); qs <- []; }
+  proc o(x:group): bits = { var y; qs <- x::qs; y <@ LRO.o(x); return y; }
+  proc hash = LRO.o
 }.
 
 (* The initial scheme *)
@@ -134,20 +115,11 @@ module S = Hashed_ElGamal(H).
    the probability of B = CDH_from_CPA(SCDH_from_CPA(A,RO)) winning CDH(B) *)
 
 section.
-<<<<<<< HEAD
 
   declare module A: Adversary [choose : `{N cA.`cchoose, #O.o : cA.`ochoose},
                                guess  : `{N cA.`cguess,  #O.o : cA.`oguess}] {-H}.
 
-  axiom guess_ll (O <: ARO {-A}) : islossless O.o => islossless A(O).guess.
-=======
-  declare module A: Adversary { LRO, Log, OnBound.G1, OnBound.G_bad }.
-
-  axiom choose_ll (O <: POracle {A}): islossless O.o => islossless A(O).choose.
-  axiom guess_ll (O <: POracle {A}) : islossless O.o => islossless A(O).guess.
-
-  local module BA = A(Bound(LRO)).
->>>>>>> origin/1.0-preview
+  axiom guess_ll (O <: POracle {-A}) : islossless O.o => islossless A(O).guess.
 
   local module G0 = {
     var gxy:group
@@ -161,157 +133,8 @@ section.
       y       <$ dt;
       gx      <- g ^ x;
       gxy     <- gx ^ y;
-<<<<<<< HEAD
       (m0,m1) <@ A(H).choose(gx);
       h       <$ dbits; 
-=======
-      (m0,m1) <@ BA.choose(gx);
-      b       <$ {0,1};
-      h       <@ H.hash(gxy);
-      c       <- (g ^ y, h +^ (b ? m1 : m0));
-      b'      <@ BA.guess(c);
-      return (b' = b);
-    }
-  }.
-
-  local equiv CPA_G0: CPA(S,BA).main ~ G0.main: ={glob A} ==> ={res}.
-  proof.
-    proc.
-    inline Hashed_ElGamal(H).kg Hashed_ElGamal(H).enc.
-    swap{1} 8 -5.
-    call (_: ={glob H, Log.qs}); first by sim.
-    wp; call (_: ={glob H}); first by sim.
-    wp; rnd.
-    call (_: ={glob H, Log.qs}); first by sim.
-    wp; do !rnd.
-    by call (_: true ==> ={glob H}); first by sim.
-  qed.
-
-  local lemma Pr_CPA_G0 &m:
-    Pr[CPA(S,BA).main() @ &m: res] = Pr[G0.main() @ &m: res]
-  by byequiv CPA_G0.
-
-  local module G1 = {
-    proc main() : bool = {
-      var m0, m1, c, b, b';
-      var x, y, h, gx, gxy;
-
-      H.init();
-      x       <$ dt;
-      y       <$ dt;
-      gx      <- g ^ x;
-      gxy     <- gx ^ y;
-      (m0,m1) <@ BA.choose(gx);
-      b       <$ {0,1};
-      h       <$ dbits;
-      c       <- (g ^ y, h +^ (b ? m1 : m0));
-      b'      <@ BA.guess(c);
-      return (b' = b);
-    }
-  }.
-
-  local module G2 = {
-    var gxy : group
-
-    proc main() : bool = {
-      var m0, m1, c, b, b';
-      var x, y, h, gx;
-
-      H.init();
-      x       <$ dt;
-      y       <$ dt;
-      gx      <- g ^ x;
-      gxy     <- gx ^ y;
-      (m0,m1) <@ BA.choose(gx);
-      b       <$ {0,1};
-      h       <$ dbits;
-      c       <- (g ^ y, h +^ (b ? m1 : m0));
-      b'      <@ BA.guess(c);
-      return G2.gxy \in Log.qs;
-    }
-  }.
-
-  local module (D : ROC.Dist) (H : POracle) = {
-    module A = A(H)
-
-    var y:t
-    var b:bool
-    var m0, m1:ptxt
-
-    proc a1(): group = {
-      var x, gxy, gx;
-
-      x       <$ dt;
-      y       <$ dt;
-      gx      <- g ^ x;
-      gxy     <- gx ^ y;
-      (m0,m1) <@ A.choose(gx);
-      b       <$ {0,1};
-      return gxy;
-    }
-
-    proc a2(x:bits): bool = {
-      var c, b';
-
-      c  <- (g ^ y, x +^ (b ? m1 : m0));
-      b' <@ A.guess(c);
-      return (b' = b);
-    }
-  }.
-
-  local lemma G0_D &m: Pr[G0.main() @ &m: res] = Pr[OnBound.G0(D,LRO).main() @ &m: res].
-  proof.
-    byequiv (_: ={glob A} ==> ={res})=> //.
-    proc.
-    inline D(Bound(LRO)).a1 D(Bound(LRO)).a2; wp.
-    conseq (_: _ ==> ={b'} /\ b{1} = D.b{2})=> //.
-    by inline H.hash; sim.
-  qed.
-
-  local lemma G1_D &m: Pr[G1.main() @ &m: res] = Pr[OnBound.G1(D,LRO).main() @ &m: res].
-  proof.
-    byequiv (_: ={glob A} ==> ={res})=> //.
-    proc.
-    inline D(Bound(LRO)).a1 D(Bound(LRO)).a2; wp.
-    conseq (_: _ ==> ={b'} /\ b{1} = D.b{2})=> //.
-    by inline H.hash; sim.
-  qed.
-
-  local lemma G2_D &m: Pr[G2.main() @ &m: res] = Pr[OnBound.G_bad(D,LRO).main() @ &m: res].
-  proof.
-    byequiv (_: ={glob A} ==> ={res})=> //.
-    proc.
-    inline D(Bound(LRO)).a1 D(Bound(LRO)).a2; wp.
-    conseq (_: _ ==> ={glob Log, b'} /\ b{1} = D.b{2} /\ G2.gxy{1} = x{2})=> //.
-    by inline H.hash; sim.
-  qed.
-
-  local lemma G0_G1_G2 &m:
-    Pr[G0.main() @ &m: res] <= Pr[G1.main() @ &m: res] + Pr[G2.main() @ &m: res].
-  proof.
-  rewrite (G0_D &m) (G1_D &m) (G2_D &m).
-  move: (OnBound.ROM_BadCall D _ _ _ &m tt true).
-  + move=> H H_o_ll; proc; auto; call (choose_ll H _)=> //; auto=> />.
-    by rewrite dt_ll DBool.dbool_ll.
-  + by move=> H H_o_ll; proc; auto; call (guess_ll H _)=> //; auto=> />.
-  + by move=> _; apply: dbits_ll.
-  by rewrite !eqT.
-  qed.
-
-  local module G1' = {
-    proc main() : bool = {
-      var m0, m1, c, b, b';
-      var x, y, h, gx, gxy;
-
-      H.init();
-      x       <$ dt;
-      y       <$ dt;
-      gx      <- g ^ x;
-      gxy     <- gx ^ y;
-      (m0,m1) <@ BA.choose(gx);
-      b       <$ {0,1};
-      h       <$ dbits;
->>>>>>> origin/1.0-preview
       c       <- (g ^ y, h);
       b'      <@ A(H).guess(c);
       b       <$ {0,1};
@@ -320,54 +143,34 @@ section.
   }.
 
   local lemma Pr_CPA_G0 &m :
-    Pr[CPA(S,A(RO)).main() @ &m: res] <= 
+    Pr[CPA(S,A(LRO)).main() @ &m: res] <= 
       Pr[G0.main() @ &m: res] + Pr[G0.main() @ &m: G0.gxy \in H.qs].
   proof.
     byequiv => //.
     proc.
-<<<<<<< HEAD
     inline Hashed_ElGamal(H).kg Hashed_ElGamal(H).enc H.hash.
     swap{1} 8 -5; swap{2} 10 -3.
     call (_: G0.gxy \in H.qs, 
-            (forall x, x \in H.qs{2} = x \in RO.m{2}) /\
-            eq_except (pred1 G0.gxy{2}) RO.m{1} RO.m{2}).
+            (forall x, x \in H.qs{2} = x \in LRO.m{2}) /\
+            eq_except (pred1 G0.gxy{2}) LRO.m{1} LRO.m{2}).
     + by apply guess_ll.
     + proc; inline *; auto => /> &1 &2 hb; smt (eq_except_set_eq get_setE).
     + by move=> *; islossless.
     + by move=> /=; proc; call (_: true); 1: islossless; auto => />.
     wp; rnd (fun y0 => y0 +^ m{1}) => /=.
-    wp; rnd; call (_: ={RO.m} /\ (forall x, x \in H.qs{2} = x \in RO.m{2})).
+    wp; rnd; call (_: ={LRO.m} /\ (forall x, x \in H.qs{2} = x \in LRO.m{2})).
     + by proc; inline *; auto => />; smt (get_setE).
     inline *; auto => /> *; split; 1: by move=> *; rewrite mem_empty.
     move=> _ ??? hdom ??; split; 1: by move=> *;ring.
     smt(eq_except_setl get_setE).
-=======
-    call (_: ={glob LRO, glob Log}); first by sim.
-    wp; rnd (fun h, h +^ if b then m1 else m0){1}; rnd.
-    call (_: ={glob LRO, glob Log}); first by sim.
-    by inline H.init LRO.init; auto=> /> *; split => *; algebra.
->>>>>>> origin/1.0-preview
   qed.
 
   local lemma Pr_G0_res &m : 
      Pr[G0.main() @ &m: res] <= 1%r/2%r.
   proof.
-<<<<<<< HEAD
     byphoare => //; proc.
     rnd (pred1 b'); conseq (_:true) => //.
     by move=> /> *; rewrite DBool.dbool1E.
-=======
-    have LRO_o_ll := LRO_o_ll _; first by move=> /=; apply: dbits_ll.
-    byphoare (_: true ==> res)=> //.
-    proc.
-    swap 7 3.
-    rnd (pred1 b').
-    conseq (_: true) => />.
-    + by move=> b'; rewrite DBool.dbool1E /pred1 => />.
-    islossless.
-    + by apply (guess_ll (Bound(LRO))); islossless.
-    by apply (choose_ll (Bound(LRO))); islossless.
->>>>>>> origin/1.0-preview
   qed.
 
   local module ALCDH = {
@@ -388,18 +191,17 @@ section.
     choare [ALCDH.solve : true ==> 0 < size res <= cA.`ochoose + cA.`oguess] 
     time [N (6 + cunifin + (3 + cunifin + cget qH + cset qH + cin qH) * (cA.`oguess + cA.`ochoose) + cA.`cguess + cA.`cchoose)].
   proof.
-<<<<<<< HEAD
     proc; wp.
-    call (_: size H.qs- cA.`ochoose <= k /\ bounded RO.m (size H.qs);
+    call (_: size H.qs- cA.`ochoose <= k /\ bounded LRO.m (size H.qs);
            time
            [(H.o k : [N(3 + cunifin + cget qH + cset qH + cin qH)])]).
     + move=> zo hzo; proc; inline *.
-      wp := (bounded RO.m qH).
+      wp := (bounded LRO.m qH).
       by rnd; auto => &hr />; rewrite dbits_ll /=; smt (cset_pos bounded_set).
-    wp; rnd; call (_: size H.qs = k /\ bounded RO.m (size H.qs);
+    wp; rnd; call (_: size H.qs = k /\ bounded LRO.m (size H.qs);
            time [(H.o k : [N(3 + cunifin + cget qH + cset qH + cin qH)])]).
     + move=> zo hzo; proc; inline *.
-      wp := (bounded RO.m qH).
+      wp := (bounded LRO.m qH).
       rnd;auto => &hr />; rewrite dbits_ll /=; smt(cset_pos bounded_set cA_pos).
     inline *; auto => />.
     split => *.
@@ -409,22 +211,9 @@ section.
 
   local lemma Pr_G0_LCDHPr_G0_res &m: 
     Pr[G0.main() @ &m: G0.gxy \in H.qs] <= Pr[LCDH(ALCDH).main() @ &m : res].
-=======
-    byequiv (_: ={glob A} ==> ={res})=> //.
-    proc.
-    call (_: ={glob LRO, glob Log}); first by sim.
-    wp; rnd (fun h, h +^ if b then m1 else m0){1}; rnd.
-    call (_: ={glob LRO, glob Log}); first by sim.
-    by inline H.init LRO.init; auto=> /> *; split => *; algebra.
-  qed.
-
-  local equiv G2'_SCDH: G2'.main ~ SCDH(SCDH_from_CPA(A,LRO)).main:
-    ={glob A} ==> res{1} = res{2} /\ card Log.qs{1} <= qH.
->>>>>>> origin/1.0-preview
   proof.
     byequiv => //.
     proc.
-<<<<<<< HEAD
     conseq (_ : _ ==> G0.gxy{1} \in H.qs{1} => g ^ (x{2} * y{2}) \in s{2}) _ (_: true ==> size s <= qH) => //.
     + by move=> />.
     + call (_: true ==> 0 < size res <= qH); last by auto.
@@ -441,35 +230,8 @@ section.
                   6 + cunifin + 
                   (3 + cunifin + cget qH + cset qH + cin qH) * (cA.`oguess + cA.`ochoose) + cA.`cguess + cA.`cchoose)}]
                {+A, +H}),
-    Pr[CPA(S,A(RO)).main() @ &m: res] - 1%r/2%r <= 
+    Pr[CPA(S,A(LRO)).main() @ &m: res] - 1%r/2%r <= 
     qH%r * Pr[CDH.CDH(B).main() @ &m: res].
-=======
-    inline SCDH_from_CPA(A,LRO).solve.
-    swap{2} 5 -4; swap{1} 7 3.
-    rnd{1}; wp.
-    seq  8  7: (={glob BA} /\
-                c{1} = (gy, h){2} /\
-                G2'.gxy{1} = g ^ (x * y){2} /\
-                card Log.qs{1} <= qH).
-      wp; rnd; call (_: ={glob H} /\ card Log.qs{1} <= qH).
-        proc; sp; if=> //; inline Log(LRO).o LRO.o; auto=> />.
-        by move=> &2 _ szqs_lt_qH _ _; rewrite fcardU fcard1; smt(fcard_ge0).
-      by inline H.init LRO.init; auto=> />; rewrite fcards0; smt(gt0_qH pow_pow).
-    call (_: ={glob H} /\ card Log.qs{1} <= qH).
-      proc; sp; if=> //; inline Log(LRO).o LRO.o; auto=> /> &2 _ szqs_lt_qH _ _.
-      by rewrite fcardU fcard1; smt(fcard_ge0).
-    by auto => />.
-  qed.
-
-  local lemma Pr_G2'_SCDH &m :
-    Pr[G2'.main() @ &m: res]
-    = Pr[SCDH(SCDH_from_CPA(A,LRO)).main() @ &m : res]
-  by byequiv G2'_SCDH.
-
-  local lemma Reduction &m :
-    Pr[CPA(S,BA).main() @ &m : res] <=
-    1%r / 2%r + Pr[SCDH(SCDH_from_CPA(A,LRO)).main() @ &m : res].
->>>>>>> origin/1.0-preview
   proof.
     have [B hB]:= C1.ex_reduction _ ALCDH &m cost_ALCDH.
     exists B; split.
@@ -477,19 +239,6 @@ section.
     move: (Pr_CPA_G0 &m) (Pr_G0_res &m) (Pr_G0_LCDHPr_G0_res) => /#.
   qed.
 
-<<<<<<< HEAD
-=======
-  (** Composing reduction from CPA to SCDH with reduction from SCDH to CDH *)
-  lemma Security &m:
-      Pr[CPA(S,A(Bound(LRO))).main() @ &m: res] - 1%r / 2%r <=
-      qH%r * Pr[CDH.CDH(CDH_from_SCDH(SCDH_from_CPA(A,LRO))).main() @ &m: res].
-  proof.
-    apply (ler_trans (Pr[SCDH(SCDH_from_CPA(A,LRO)).main() @ &m: res])).
-    + smt(Reduction).
-    have:= Self.SCDH.Reduction (SCDH_from_CPA(A,LRO)) &m gt0_qH.    
-    by rewrite -mulrA mul1r mulrC ler_pdivr_mulr 1:lt_fromint 1:gt0_qH mulrC.
-  qed.
->>>>>>> origin/1.0-preview
 end section.
 
 print ex_reduction.
